\documentclass[10pt,a4paper]{article}
\usepackage[utf8]{inputenc}
\usepackage{amsmath}
\usepackage{amsfonts}
\usepackage{amssymb}
\usepackage{mathrsfs} %花体字母
\begin{document}


\begin{equation}
J_{(\theta)} = -\frac{1}{m} \left[ \sum_{i=1}^m \sum_{j=1}^k {\omega}_{j} \log{\frac{\exp({{\theta}_j^{T}x^{(i)}})}{\sum_{l=1}^k{ \exp({{\theta}_l^{T}x^{(i)}})}} } \right]
\end{equation}

\begin{equation}
J{(\theta)} = -\frac{1}{m} \sum_{i=1}^m \omega \left[ y^{(i)} \log{(h_{\theta}(x^{(i)}))} + ( 1 - y^{(i)}) \log{(1- h_{\theta}(x^{(i)}))} \right]
\end{equation}
 
\begin{equation}
\omega = \left\{\begin{array}{11}
 10 & \forall p(i,j) \in \mathbf{E} \\
  1  & otherwise
  \right.
\end{array}       
\end{equation}

\end{document}